Readme.md
@@ -1,3 +1,4 @@
-The current version works only on Isabelle-2021, but we will migrate to the latest Isabeele-2021-1 soon.
+The current version works only on Isabelle-2021 (*not* Isabelle-2021-1), but we will migrate to the latest Isabelle-2021-1 soon.
 
-Some special symbols are required. Please put contents in the file `symbols` into your Isabelle symbol file `$HOME/.isabelle/Isabelle2021/etc/symbols`.
+Some additional symbols are required. Please copy lines in the file `symbols` into your Isabelle symbol file `$HOME/.isabelle/Isabelle2021/etc/symbols`.
+You may also need to install the Symbola font which is given in the directory `fonts`.
